LL1/ParserTests.v
@@ -4,39 +4,19 @@ Require Import Lib.ExampleGrammars.
 Require Import Lib.Grammar.
 Require Import Lib.ParseTree.
 
+Require Import LL1.ExampleParseTables.
 Require Import LL1.Parser.
 Require Import LL1.ParseTable.
 
 Import ListNotations.
 
-Example test1 :
+Example g311_test :
   parse g311ParseTable (NT X) g311Sentence1 100 =
   (Some g311ParseTree1, nil).
-Proof. simpl. reflexivity. Qed.
-
-Definition x_y_grammar :=
-  [(NT X, [NT Y]);
-     (NT Y, [])].
-
-Definition x_map := 
-  LaMap.add 
-    EOF [NT Y]
-    (LaMap.empty (list symbol)).
-
-Definition y_map := 
-  LaMap.add 
-    EOF nil
-    (LaMap.empty (list symbol)).
-
-Definition x_y_parse_table :=
-  NtMap.add
-    X x_map
-    (NtMap.add
-       Y y_map
-       (NtMap.empty (LaMap.t (list symbol)))).
+Proof. auto. Qed.
                 
-Example x_y_test1 :
-  parse x_y_parse_table (NT X) nil 100 =
+Example xy_test :
+  parse xy_parse_table (NT X) nil 100 =
   (Some (Node X [Node Y []]), nil).
 Proof. auto. Qed.
 
